



$$Z = \frac{e}{i_d} \quad \text{pero } i_d = g_m v_g$$

$$v_g = \frac{R}{R - jX_c} e$$

entonces:

$$Z = \frac{e}{g_m \left(\frac{R}{R - jX_c} e \right)} = \frac{R - jX_c}{g_m R}$$

$$Z = \frac{1}{g_m} - j \frac{X_c}{g_m R}$$

si $R \ll X_c$

entonces:

$$Z \approx -j \frac{X_c}{g_m R} = -j \frac{1}{g_m (2\pi f_0 C) R}$$

$$Z = -j \frac{1}{2\pi f_0 C_{eq}}$$

$$\text{donde } C_{eq} = g_m R C$$

$$g_m = \frac{2I_{DSS}}{V_{GS}} \left(1 - \frac{V_{GS}}{V_{GS0}} \right)$$

Para TBJ se sigue el mismo procedimiento, resultando:

$$Z = -j \frac{1}{2\pi f_0 C_{eq}}$$

$$\text{donde } C_{eq} = \frac{\beta R C}{\beta R e + R}$$